feat: faster, linear HashMap.alter and modify (#6573)
This PR replaces the existing implementations of `(D)HashMap.alter` and
`(D)HashMap.modify` with primitive, more efficient ones and in
particular provides proofs that they yield well-formed hash maps (`WF`
typeclass).

---------

Co-authored-by: Paul Reichert <6992158+datokrat@users.noreply.github.com>

src/Std/Data/HashMap/Basic.lean
@@ -245,21 +245,13 @@ instance [BEq α] [Hashable α] {m : Type w → Type w} : ForIn m (HashMap α β
     Array β :=
   m.inner.valuesArray
 
-@[inline, inherit_doc DHashMap.modify] def modify (m : HashMap α β) (a : α) (f : β → β) : HashMap α β :=
-  match m.get? a with
-  | none => m
-  | some b => m.erase a |>.insert a (f b)
+@[inline, inherit_doc DHashMap.modify] def modify (m : HashMap α β) (a : α) (f : β → β) :
+    HashMap α β :=
+  ⟨DHashMap.Const.modify m.inner a f⟩
 
-@[inline, inherit_doc DHashMap.alter] def alter (m : HashMap α β) (a : α) (f : Option β → Option β) : HashMap α β :=
-  match m.get? a with
-  | none =>
-    match f none with
-    | none => m
-    | some b => m.insert a b
-  | some b =>
-    match f (some b) with
-    | none => m.erase a
-    | some b => m.erase a |>.insert a b
+@[inline, inherit_doc DHashMap.alter] def alter (m : HashMap α β) (a : α)
+    (f : Option β → Option β) : HashMap α β :=
+  ⟨DHashMap.Const.alter m.inner a f⟩
 
 @[inline, inherit_doc DHashMap.Const.insertMany] def insertMany {ρ : Type w}
     [ForIn Id ρ (α × β)] (m : HashMap α β) (l : ρ) : HashMap α β :=
