src/Std/Data/DHashMap/Internal/Model.lean
@@ -41,6 +41,11 @@ def bucket [Hashable α] (self : Array (AssocList α β)) (h : 0 < self.size) (k
   let ⟨i, h⟩ := mkIdx self.size h (hash k)
   self[i]
 
+theorem bucket_eq {α : Type u} {β : α → Type v} [Hashable α] (self : Array (AssocList α β))
+  (h : 0 < self.size) (k : α) : bucket self h k =
+    haveI := mkIdx self.size h (hash k) |>.2
+    self[mkIdx self.size h (hash k) |>.1] := rfl
+
 /-- Internal implementation detail of the hash map -/
 def updateBucket [Hashable α] (self : Array (AssocList α β)) (h : 0 < self.size) (k : α)
     (f : AssocList α β → AssocList α β) : Array (AssocList α β) :=
@@ -78,6 +83,13 @@ theorem size_withComputedSize {self : Array (AssocList α β)} :
 @[simp]
 theorem buckets_withComputedSize {self : Array (AssocList α β)} :
     (withComputedSize self).buckets = self := rfl
+
+@[simp]
+theorem bucket_updateBucket [Hashable α] (self : Array (AssocList α β)) (h : 0 < self.size) (k : α)
+    (f : AssocList α β → AssocList α β) :
+    bucket (updateBucket self h k f) (by simpa using h) k = f (bucket self h k) := by
+  unfold bucket updateBucket mkIdx
+  simp
 
 theorem exists_bucket_of_uset [BEq α] [Hashable α]
   (self : Array (AssocList α β)) (i : USize) (hi : i.toNat < self.size) (d : AssocList α β) :
@@ -165,13 +177,14 @@ theorem apply_bucket_with_proof {γ : α → Type w} [BEq α] [Hashable α] [Par
 /-- This is the general theorem to show that modification operations are correct. -/
 theorem toListModel_updateBucket [BEq α] [Hashable α] [PartialEquivBEq α] [LawfulHashable α]
     {m : Raw₀ α β} (hm : Raw.WFImp m.1) {a : α} {f : AssocList α β → AssocList α β}
-    {g : List ((a : α) × β a) → List ((a : α) × β a)} (hfg : ∀ {l}, (f l).toList = g l.toList)
+    {g : List ((a : α) × β a) → List ((a : α) × β a)} (hfg : ∀ {l}, Perm (f l).toList (g l.toList))
     (hg₁ : ∀ {l l'}, DistinctKeys l → Perm l l' → Perm (g l) (g l'))
     (hg₂ : ∀ {l l'}, containsKey a l' = false → g (l ++ l') = g l ++ l') :
     Perm (toListModel (updateBucket m.1.buckets m.2 a f)) (g (toListModel m.1.2)) := by
   obtain ⟨l, h₁, h₂, h₃⟩ := exists_bucket_of_update m.1.buckets m.2 a f
   refine h₂.trans (Perm.trans ?_ (hg₁ hm.distinct h₁).symm)
-  rw [hfg, hg₂]
+  refine Perm.append_right l hfg |>.trans ?_
+  rw [hg₂]
   exact h₃ hm.buckets_hash_self _ rfl
 
 /-- This is the general theorem to show that mapping operations (like `map` and `filter`) are
@@ -311,6 +324,49 @@ def eraseₘ [BEq α] [Hashable α] (m : Raw₀ α β) (a : α) : Raw₀ α β :
   if m.containsₘ a then m.eraseₘaux a else m
 
 /-- Internal implementation detail of the hash map -/
+def alterₘ [BEq α] [Hashable α] [LawfulBEq α] (m : Raw₀ α β) (a : α)
+    (f : Option (β a) → Option (β a)) : Raw₀ α β :=
+  if h : m.containsₘ a then
+    let buckets' := updateBucket m.1.buckets m.2 a (fun l => l.alter a f)
+    let size' :=
+      if Raw₀.containsₘ ⟨withComputedSize buckets', by simpa [buckets'] using m.2⟩ a
+      then m.1.size else m.1.size - 1
+    ⟨⟨size', buckets'⟩, by simpa [buckets'] using m.2⟩
+  else
+    match f none with
+    | none => m
+    | some b => Raw₀.expandIfNecessary (m.consₘ a b)
+
+/-- Internal implementation detail of the hash map -/
+def modifyₘ [BEq α] [Hashable α] [LawfulBEq α] (m : Raw₀ α β) (a : α) (f : β a → β a) : Raw₀ α β :=
+  m.alterₘ a (·.map f)
+
+namespace Const
+
+variable {β : Type v}
+
+/-- Internal implementation detail of the hash map -/
+def alterₘ [BEq α] [Hashable α] (m : Raw₀ α (fun _ => β)) (a : α)
+    (f : Option β → Option β) : Raw₀ α (fun _ => β) :=
+  if h : m.containsₘ a then
+    let buckets' := updateBucket m.1.buckets m.2 a (fun l => AssocList.Const.alter a f l)
+    let size' :=
+      if Raw₀.containsₘ ⟨withComputedSize buckets', by simpa [buckets'] using m.2⟩ a
+      then m.1.size else m.1.size - 1
+    ⟨⟨size', buckets'⟩, by simpa [buckets'] using m.2⟩
+  else
+    match f none with
+    | none => m
+    | some b => Raw₀.expandIfNecessary (m.consₘ a b)
+
+/-- Internal implementation detail of the hash map -/
+def modifyₘ [BEq α] [Hashable α] (m : Raw₀ α (fun _ => β)) (a : α) (f : β → β) :
+    Raw₀ α (fun _ => β) :=
+  alterₘ m a (fun option => option.map f)
+
+end Const
+
+/-- Internal implementation detail of the hash map -/
 def filterMapₘ (m : Raw₀ α β) (f : (a : α) → β a → Option (δ a)) : Raw₀ α δ :=
   ⟨withComputedSize (updateAllBuckets m.1.buckets fun l => l.filterMap f), by simpa using m.2⟩
 
@@ -390,6 +446,64 @@ theorem insert_eq_insertₘ [BEq α] [Hashable α] (m : Raw₀ α β) (a : α) (
     rw [Array.set_set, updateBucket]
     simp only [Array.uset, Array.ugetElem_eq_getElem]
   · rfl
+
+theorem alter_eq_alterₘ [BEq α] [Hashable α] [LawfulBEq α] (m : Raw₀ α β) (a : α)
+    (f : Option (β a) → Option (β a)) : m.alter a f = m.alterₘ a f := by
+    dsimp only [alter, alterₘ, containsₘ, ← bucket_eq]
+    split
+    · congr 2
+      · simp only [withComputedSize, bucket_updateBucket]
+      · simp only [Array.uset, bucket, Array.ugetElem_eq_getElem, Array.set_set, updateBucket]
+    · congr
+
+theorem modify_eq_alter [BEq α] [Hashable α] [LawfulBEq α] (m : Raw₀ α β) (a : α)
+    (f : β a → β a) : m.modify a f = m.alter a (·.map f) := by
+  rw [modify, alter]
+  split
+  · dsimp
+    split
+    · next h =>
+      simp only [AssocList.contains_eq] at h
+      simp only [AssocList.modify_eq_alter, Array.set_set, AssocList.contains_eq,
+        containsKey_of_perm AssocList.toList_alter, ← modifyKey_eq_alterKey,
+        containsKey_modifyKey_self, h, ↓reduceIte]
+    · rfl
+
+theorem modify_eq_modifyₘ [BEq α] [Hashable α] [LawfulBEq α] (m : Raw₀ α β) (a : α)
+    (f : β a → β a) : m.modify a f = m.modifyₘ a f := by
+  rw [modify_eq_alter, alter_eq_alterₘ, modifyₘ]
+
+namespace Const
+
+variable {β : Type v}
+
+theorem alter_eq_alterₘ [BEq α] [Hashable α] [EquivBEq α] (m : Raw₀ α (fun _ => β)) (a : α)
+    (f : Option β → Option β) : Const.alter m a f = Const.alterₘ m a f := by
+    dsimp only [alter, alterₘ, containsₘ, ← bucket_eq]
+    split
+    · congr 2
+      · simp only [withComputedSize, bucket_updateBucket]
+      · simp only [Array.uset, bucket, Array.ugetElem_eq_getElem, Array.set_set, updateBucket]
+    · congr
+
+theorem modify_eq_alter [BEq α] [Hashable α] [EquivBEq α] (m : Raw₀ α (fun _ => β)) (a : α)
+    (f : β → β) : Const.modify m a f = Const.alter m a (·.map f) := by
+  rw [modify, alter]
+  split
+  · dsimp
+    split
+    · next h =>
+      simp only [AssocList.contains_eq] at h
+      simp only [AssocList.Const.modify_eq_alter, Array.set_set, AssocList.contains_eq,
+        containsKey_of_perm AssocList.Const.toList_alter, ← Const.modifyKey_eq_alterKey,
+        Const.containsKey_modifyKey_self, h, ↓reduceIte]
+    · rfl
+
+theorem modify_eq_modifyₘ [BEq α] [Hashable α] [EquivBEq α] (m : Raw₀ α (fun _ => β)) (a : α)
+    (f : β → β) : Const.modify m a f = Const.modifyₘ m a f := by
+  rw [modify_eq_alter, alter_eq_alterₘ, modifyₘ]
+
+end Const
 
 theorem containsThenInsert_eq_insertₘ [BEq α] [Hashable α] (m : Raw₀ α β) (a : α) (b : β a) :
     (m.containsThenInsert a b).2 = m.insertₘ a b := by
